wip on matchIndex allEntries

raft-proofs/MatchIndexAllEntriesProof.v
@@ -1,4 +1,5 @@
 Require Import List.
+Require Import Omega.
 
 Require Import VerdiTactics.
 Require Import Net.
@@ -6,8 +7,21 @@ Require Import Util.
 Require Import Raft.
 Require Import RaftRefinementInterface.
 
-Require Import MatchIndexAllEntriesInterface.
+Require Import CommonTheorems.
+Require Import RefinementCommonTheorems.
+Require Import SpecLemmas.
+Require Import RefinementSpecLemmas.
 
+Require Import UpdateLemmas.
+Local Arguments update {_} {_} {_} _ _ _ _ : simpl never.
+
+Require Import NoAppendEntriesToLeaderInterface.
+Require Import NoAppendEntriesToSelfInterface.
+Require Import TermsAndIndicesFromOneLogInterface.
+Require Import RefinedLogMatchingLemmasInterface.
+Require Import LogAllEntriesInterface.
+
+Require Import MatchIndexAllEntriesInterface.
 
 Section MatchIndexAllEntries.
   Context {orig_base_params : BaseParams}.
@@ -16,7 +30,514 @@ Section MatchIndexAllEntries.
 
   Context {rri : raft_refinement_interface}.
 
-  Instance miaei : match_index_all_entries_interface.
+  Context {naetli : no_append_entries_to_leader_interface}.
+  Context {naetsi : no_append_entries_to_self_interface}.
+  Context {taifoli : terms_and_indices_from_one_log_interface}.
+  Context {rlmli : refined_log_matching_lemmas_interface}.
+  Context {laei : log_all_entries_interface}.
+
+  Definition match_index_all_entries_nw (net : network) : Prop :=
+    forall p t es e,
+      In p (nwPackets net) ->
+      pBody p = AppendEntriesReply t es true ->
+      currentTerm (snd (nwState net (pDst p))) = t ->
+      In e (log (snd (nwState net (pDst p)))) ->
+      eTerm e = t ->
+      eIndex e <= maxIndex es ->
+      type (snd (nwState net (pDst p))) = Leader ->
+      In (t, e) (allEntries (fst (nwState net (pSrc p)))).
+
+  Definition match_index_all_entries_inv (net : network) : Prop :=
+    match_index_all_entries net /\ match_index_all_entries_nw net.
+
+  Lemma match_index_all_entries_init :
+    refined_raft_net_invariant_init match_index_all_entries_inv.
+  Proof.
+    unfold refined_raft_net_invariant_init,
+           match_index_all_entries_inv,
+           match_index_all_entries_nw,
+           match_index_all_entries.
+    simpl. intros.
+    intuition.
+  Qed.
+
+  Ltac update_destruct :=
+    match goal with
+      | [ H : context [ update _ ?x _ ?y ] |- _ ] =>
+        destruct (name_eq_dec x y); subst; rewrite_update; simpl in *
+      | [ |- context [ update _ ?x _ ?y ] ] =>
+        destruct (name_eq_dec x y); subst; rewrite_update; simpl in *
+    end.
+
+  Lemma match_index_all_entries_client_request :
+    refined_raft_net_invariant_client_request match_index_all_entries_inv.
   Admitted.
 
-End MatchIndexAllEntries.  
+  Lemma match_index_all_entries_timeout :
+    refined_raft_net_invariant_timeout match_index_all_entries_inv.
+  Admitted.
+
+  Lemma handleAppendEntries_post_leader_nop :
+    forall h st t n pli plt es ci st' m,
+      currentTerm st <> t ->
+      handleAppendEntries h st t n pli plt es ci = (st', m) ->
+      type st' = Leader ->
+      st' = st.
+  Proof.
+    unfold handleAppendEntries.
+    intros.
+    repeat break_match; repeat find_inversion; auto; try discriminate.
+  Qed.
+
+  Lemma handleAppendEntries_leader_was_leader :
+    forall h st t n pli plt es ci st' m,
+      handleAppendEntries h st t n pli plt es ci = (st', m) ->
+      type st' = Leader ->
+      type st = Leader.
+  Proof.
+    unfold handleAppendEntries.
+    intros.
+    repeat break_match; repeat find_inversion; auto; try discriminate.
+  Qed.
+
+  Lemma ghost_packet :
+    forall (net : network (params := raft_refined_multi_params)) p,
+      In p (nwPackets net) ->
+      In (deghost_packet p) (nwPackets (deghost net)).
+  Proof.
+    unfold deghost.
+    simpl. intuition.
+    apply in_map_iff.
+    eexists; eauto.
+  Qed.
+
+  Lemma pDst_deghost_packet :
+    forall p : packet (params := raft_refined_multi_params),
+      pDst (deghost_packet p) = pDst p.
+  Proof.
+    unfold deghost_packet. auto.
+  Qed.
+
+  Lemma lifted_no_AE_to_leader :
+    forall net p t n pli plt es ci,
+      refined_raft_intermediate_reachable net ->
+      In p (nwPackets net) ->
+      pBody p = AppendEntries t n pli plt es ci ->
+      type (snd (nwState net (pDst p))) = Leader ->
+      currentTerm (snd (nwState net (pDst p))) = t ->
+      False.
+  Proof.
+    intros.
+    pose proof (lift_prop _ no_append_entries_to_leader_invariant _ $(eauto)$).
+    unfold no_append_entries_to_leader in *.
+    find_apply_lem_hyp ghost_packet.
+    match goal with
+    | [ H : forall _ _ _ , _, H' : In _ _ |- _ ] => eapply H in H'; eauto
+    end;
+    rewrite deghost_spec;
+    rewrite pDst_deghost_packet; auto.
+  Qed.
+
+  Lemma lifted_no_AE_to_self :
+    forall net p t n pli plt es ci,
+      refined_raft_intermediate_reachable net ->
+      In p (nwPackets net) ->
+      pBody p = AppendEntries t n pli plt es ci ->
+      pDst p = pSrc p ->
+      False.
+  Proof.
+    intros.
+    pose proof (lift_prop _ no_append_entries_to_self_invariant _ $(eauto)$).
+    unfold no_append_entries_to_self in *.
+    find_apply_lem_hyp ghost_packet.
+    match goal with
+    | [ H : forall _ _ _ , _, H' : In _ _ |- _ ] => eapply H in H'; eauto
+    end.
+  Qed.
+
+  Lemma handleAppendEntries_message :
+    forall h st t n pli plt es ci st' m,
+      handleAppendEntries h st t n pli plt es ci = (st', m) ->
+      exists res, m = AppendEntriesReply (currentTerm st') es res.
+  Proof.
+    unfold handleAppendEntries, advanceCurrentTerm.
+    intros. repeat break_match; repeat find_inversion; simpl in *; repeat do_bool; eauto;
+            eexists; f_equal; eauto using NPeano.Nat.le_antisymm.
+  Qed.
+
+  Lemma not_empty_true_elim :
+    forall A (l : list A),
+      not_empty l = true -> l <> nil.
+  Proof.
+    unfold not_empty.
+    intros. break_match; congruence.
+  Qed.
+
+  Lemma not_empty_false_elim :
+    forall A (l : list A),
+      not_empty l = false -> l = nil.
+  Proof.
+    unfold not_empty.
+    intros. break_match; congruence.
+  Qed.
+
+  Lemma handleAppendEntries_success_allEntries :
+    forall h st t n pli plt es ci st' t',
+      handleAppendEntries h st t n pli plt es ci = (st', AppendEntriesReply t' es true) ->
+      es <> nil ->
+      (forall e e' e'',
+          In e es ->
+          In e' (log st) ->
+          eIndex e = eIndex e' ->
+          eTerm e = eTerm e' ->
+          In e'' es ->
+          eIndex e'' <= eIndex e ->
+          In e'' (log st)) ->
+      sorted (log st) ->
+      exists e, In e (log st') /\ In e es /\
+                eIndex e = maxIndex es /\
+                eTerm e = maxTerm es.
+  Proof.
+    unfold handleAppendEntries, haveNewEntries.
+    intros.
+    break_if; try find_inversion.
+    break_if.
+    - break_if; find_inversion; simpl;
+      repeat (do_bool; repeat break_and).
+      + find_apply_lem_hyp not_empty_true_elim.
+        pose proof maxIndex_non_empty es $(auto)$.
+        break_exists_exists. intuition.
+      + break_or_hyp.
+        * find_apply_lem_hyp not_empty_false_elim. congruence.
+        * break_match; try discriminate.
+          do_bool. rewrite advanceCurrentTerm_log.
+          find_apply_lem_hyp findAtIndex_elim. break_and.
+          pose proof maxIndex_non_empty es $(auto)$.
+          break_exists_name e'. break_and.
+          match goal with
+          | [ H : forall _ _ _, In _ _ -> _ |- _ ] =>
+            specialize (H e' e e')
+          end.
+          repeat find_rewrite. repeat concludes. intuition.
+          assert (e = e').
+          { eapply uniqueIndices_elim_eq; eauto.
+            auto using sorted_uniqueIndices.
+          }
+          subst. eauto.
+    - break_match; try find_inversion.
+      break_if; try find_inversion.
+      break_if; find_inversion; simpl;
+      repeat (do_bool; repeat break_and).
+      + find_apply_lem_hyp not_empty_true_elim.
+        pose proof maxIndex_non_empty es $(auto)$.
+        break_exists_exists. intuition.
+      + break_or_hyp.
+        * find_apply_lem_hyp not_empty_false_elim. congruence.
+        * break_match; try discriminate.
+          do_bool. rewrite advanceCurrentTerm_log.
+          find_apply_lem_hyp findAtIndex_elim. break_and.
+          pose proof maxIndex_non_empty es $(auto)$.
+          break_exists_name e'. break_and.
+          match goal with
+          | [ H : forall _ _ _, In _ _ -> _ |- _ ] =>
+            specialize (H e' e0 e')
+          end.
+          repeat find_rewrite. repeat concludes. intuition.
+          assert (e0 = e').
+          { eapply uniqueIndices_elim_eq; eauto.
+            auto using sorted_uniqueIndices.
+          }
+          subst. eauto.
+  Qed.
+
+  Lemma handleAppendEntries_success_term :
+    forall h st t n pli plt es ci st' t',
+      handleAppendEntries h st t n pli plt es ci = (st', AppendEntriesReply t' es true) ->
+      currentTerm st' = t.
+  Proof.
+    unfold handleAppendEntries, advanceCurrentTerm.
+    intros. repeat break_match; repeat find_inversion; simpl; auto; repeat do_bool;
+    eauto using Nat.le_antisymm.
+  Qed.
+
+  Lemma lifted_terms_and_indices_from_one_log : forall net h,
+    refined_raft_intermediate_reachable net ->
+    terms_and_indices_from_one (log (snd (nwState net h))).
+  Proof.
+    intros.
+    pose proof (lift_prop _ terms_and_indices_from_one_log_invariant).
+    unfold terms_and_indices_from_one_log in *.
+    rewrite <- deghost_spec with (net0 := net). auto.
+  Qed.
+
+  Lemma maxIndex_gt_0_nonempty :
+    forall es,
+      0 < maxIndex es ->
+      es <> nil.
+  Proof.
+    intros.
+    destruct es; simpl in *.
+    - omega.
+    - congruence.
+  Qed.
+
+  Lemma appendEntries_sublog :
+    forall net p t n pli plt es ci h e,
+      refined_raft_intermediate_reachable net ->
+      In p (nwPackets net) ->
+      pBody p = AppendEntries t n pli plt es ci ->
+      currentTerm (snd (nwState net h)) = t ->
+      In e es ->
+      In e (log (snd (nwState net h))).
+  Admitted.
+
+  Lemma match_index_all_entries_append_entries :
+    refined_raft_net_invariant_append_entries' match_index_all_entries_inv.
+  Proof.
+    unfold refined_raft_net_invariant_append_entries', match_index_all_entries_inv.
+    simpl. intros. break_and.
+    split.
+    - admit.
+    - unfold match_index_all_entries_nw. simpl.  intros.
+      find_apply_hyp_hyp. break_or_hyp.
+      + unfold match_index_all_entries_nw in *.
+        repeat find_higher_order_rewrite.
+        update_destruct.
+        * assert (currentTerm (snd (nwState net (pDst p))) <> t).
+          { intro.
+            match goal with
+            | [ H : pBody _ = AppendEntries _ _ _ _ _ _ |- _ ] =>
+              eapply lifted_no_AE_to_leader with (net := net) in H; eauto
+            end.
+            eapply handleAppendEntries_leader_was_leader; eauto.
+          }
+          match goal with
+          | [ H : context [handleAppendEntries] |- _ ] =>
+            apply handleAppendEntries_post_leader_nop in H; auto
+          end.
+          subst.
+          match goal with
+          | [ H : In _ (_ ++ _), H' : forall _ _ _ _, In _ _ -> _ |- _ ] =>
+            eapply in_middle_insert in H; eapply H' in H; eauto; try congruence
+          end.
+          { update_destruct.
+            - apply update_elections_data_appendEntries_preserves_allEntries.
+              repeat find_rewrite. auto.
+            - auto.
+          }
+        * match goal with
+          | [ H : forall _ _ _ _, In _ _ -> _, H' : pBody _ = AppendEntriesReply _ _ _ |- _ ] =>
+            eapply H in H'; eauto
+          end.
+          { update_destruct.
+            - apply update_elections_data_appendEntries_preserves_allEntries.
+              repeat find_rewrite. auto.
+            - auto.
+          }
+      + simpl in *.
+        find_copy_apply_lem_hyp handleAppendEntries_message. break_exists.
+        subst. find_inversion.
+        repeat find_higher_order_rewrite.
+        update_destruct.
+        * exfalso. eapply lifted_no_AE_to_self with (net := net); eauto.
+        * unfold update_elections_data_appendEntries. repeat find_rewrite. simpl.
+          { find_copy_apply_lem_hyp handleAppendEntries_success_allEntries.
+            - break_exists. break_and.
+              find_copy_apply_lem_hyp handleAppendEntries_success_term.
+              assert (In x (log (snd (nwState net (pSrc p))))).
+              { eapply appendEntries_sublog; eauto. subst. repeat find_rewrite. auto. }
+              assert (entries_match (log d) (log (snd (nwState net (pSrc p))))).
+              { match goal with
+                | [ H : refined_raft_intermediate_reachable (mkNetwork ?a ?b) |- _ ] =>
+                  let H' := fresh "H" in
+                  pose proof entries_match_invariant _ (pDst p) (pSrc p) H as H';
+                    simpl in H'; repeat find_higher_order_rewrite; rewrite_update;
+                    simpl in H'; auto
+                end.
+              }
+              assert (In e (log d)) as Helogd.
+              { match goal with
+                | [ H : entries_match _ _ |- _ ] =>
+                  specialize (H x x e)
+                end.
+                repeat concludes. intuition.
+              }
+
+              match goal with
+              | [ H : refined_raft_intermediate_reachable (mkNetwork ?a ?b) |- _ ] =>
+                let H' := fresh "H" in
+                pose proof log_all_entries_invariant _ H (pDst p) e as H';
+                  simpl in H'; repeat find_higher_order_rewrite; rewrite_update;
+                  simpl in H'; unfold update_elections_data_appendEntries in H';
+                  repeat find_rewrite; simpl in H'
+              end.
+              auto.
+            - find_apply_lem_hyp lifted_terms_and_indices_from_one_log; auto. break_and.
+              apply maxIndex_gt_0_nonempty. omega.
+            - intros.
+              match goal with
+              | [ H : refined_raft_intermediate_reachable (mkNetwork _ _) |- _ ] => clear H
+              end.
+              pose proof entries_match_nw_host_invariant _ $(eauto)$ _ _ _ _ _ _ _ (pDst p)
+                   e0 e' e'' $(eauto)$ $(eauto)$.
+              repeat find_rewrite. auto.
+            - apply entries_sorted_invariant. auto.
+          }
+  Admitted.
+
+  Lemma handleAppendEntriesReply_spec :
+    forall n st src t es b st' l,
+      handleAppendEntriesReply n st src t es b = (st', l) ->
+      (type st' = type st /\
+       matchIndex st' = matchIndex st /\
+       currentTerm st' = currentTerm st) \/
+      (currentTerm st' = t /\ type st' = Follower) \/
+      (b = true /\
+       t = currentTerm st' /\
+       type st' = type st /\
+       matchIndex st' = assoc_set name_eq_dec (matchIndex st) src
+                                  (PeanoNat.Nat.max
+                                     (assoc_default name_eq_dec (matchIndex st) src 0) (maxIndex es)) /\
+       currentTerm st' = currentTerm st).
+  Proof.
+    unfold handleAppendEntriesReply.
+    intros.
+    repeat break_match; repeat find_inversion; simpl in *; auto.
+    - do_bool. intuition.
+    - unfold advanceCurrentTerm. break_match; auto.
+  Qed.
+
+  Lemma update_nop_fst :
+    forall A B f x (v2 : B) y,
+      fst (update f x (fst (f x), v2) y) = fst (A := A) (f y).
+  Proof.
+    intros.
+    update_destruct; auto.
+  Qed.
+
+  Lemma get_set_diff_default :
+    forall K V K_eq_dec (k k' : K) (v : V) l d,
+      k <> k' ->
+      assoc_default K_eq_dec (assoc_set K_eq_dec l k v) k' d = assoc_default K_eq_dec l k' d.
+  Proof.
+    unfold assoc_default.
+    intros.
+    repeat break_match; auto;
+    rewrite get_set_diff in * by auto; congruence.
+  Qed.
+
+  Lemma get_set_same_default :
+    forall K V K_eq_dec (k : K) (v : V) l d,
+      assoc_default K_eq_dec (assoc_set K_eq_dec l k v) k d = v.
+  Proof.
+    unfold assoc_default.
+    intros.
+    repeat break_match; auto;
+    rewrite get_set_same in *; congruence.
+  Qed.
+
+  Lemma match_index_all_entries_append_entries_reply :
+    refined_raft_net_invariant_append_entries_reply match_index_all_entries_inv.
+  Proof.
+    unfold refined_raft_net_invariant_append_entries_reply, match_index_all_entries_inv.
+    simpl. intros. split.
+    - { unfold match_index_all_entries in *. simpl. intros. break_and.
+        repeat find_higher_order_rewrite.
+        rewrite update_nop_fst.
+        update_destruct.
+        - find_copy_apply_lem_hyp handleAppendEntriesReply_spec.
+          intuition.
+          + match goal with
+            | [ H : forall _ _ _, type _ = _ -> _ |- _ ] => specialize (H e (pDst p) h)
+            end.
+            repeat find_rewrite. repeat concludes.
+            find_erewrite_lem handleAppendEntriesReply_log.
+            auto.
+          + congruence.
+          + repeat find_rewrite.
+            match goal with
+            | [ H : context [ assoc_default _ (assoc_set _ _ ?x _) ?y _ ]  |- _ ] =>
+              destruct (name_eq_dec x y)
+            end.
+            * subst. rewrite get_set_same_default in *.
+              find_apply_lem_hyp app_cons_in.
+              find_erewrite_lem handleAppendEntriesReply_log.
+              { find_apply_lem_hyp PeanoNat.Nat.max_le. break_or_hyp.
+                - match goal with
+                  | [ H : forall _ _ _, type _ = _ -> _ |- _ ] => specialize (H e (pDst p) (pSrc p))
+                  end. repeat find_rewrite. auto.
+                - unfold match_index_all_entries_nw in *.
+                  match goal with
+                  | [ H : pBody _ = _, H' : _  |- _ ] => eapply H' with (e := e) in H; auto
+                  end.
+              }
+            * rewrite get_set_diff_default in * by auto.
+              match goal with
+              | [ H : forall _ _ _, type _ = _ -> _ |- _ ] => specialize (H e (pDst p) h)
+              end.
+              repeat find_rewrite. repeat concludes.
+              find_erewrite_lem handleAppendEntriesReply_log.
+              auto.
+        - find_apply_hyp_hyp. congruence.
+      }
+    - admit.
+  Admitted.
+
+  Lemma match_index_all_entries_request_vote :
+    refined_raft_net_invariant_request_vote match_index_all_entries_inv.
+  Admitted.
+
+  Lemma match_index_all_entries_request_vote_reply :
+    refined_raft_net_invariant_request_vote_reply match_index_all_entries_inv.
+  Admitted.
+
+  Lemma match_index_all_entries_do_leader :
+    refined_raft_net_invariant_do_leader match_index_all_entries_inv.
+  Admitted.
+
+  Lemma match_index_all_entries_do_generic_server :
+    refined_raft_net_invariant_do_generic_server match_index_all_entries_inv.
+  Admitted.
+
+  Lemma match_index_all_entries_state_same_packet_subset :
+    refined_raft_net_invariant_state_same_packet_subset match_index_all_entries_inv.
+  Admitted.
+
+  Lemma match_index_all_entries_reboot :
+    refined_raft_net_invariant_reboot match_index_all_entries_inv.
+  Admitted.
+
+  Lemma match_index_all_entries_invariant :
+    forall net,
+      refined_raft_intermediate_reachable net ->
+      match_index_all_entries_inv net.
+  Proof.
+    intros.
+    apply refined_raft_net_invariant'; auto.
+    - apply match_index_all_entries_init.
+    - apply refined_raft_net_invariant_client_request'_weak.
+      apply match_index_all_entries_client_request.
+    - apply refined_raft_net_invariant_timeout'_weak.
+      apply match_index_all_entries_timeout.
+    - apply match_index_all_entries_append_entries.
+    - apply refined_raft_net_invariant_append_entries_reply'_weak.
+      apply match_index_all_entries_append_entries_reply.
+    - apply refined_raft_net_invariant_request_vote'_weak.
+      apply match_index_all_entries_request_vote.
+    - apply refined_raft_net_invariant_request_vote_reply'_weak.
+      apply match_index_all_entries_request_vote_reply.
+    - apply refined_raft_net_invariant_do_leader'_weak.
+      apply match_index_all_entries_do_leader.
+    - apply refined_raft_net_invariant_do_generic_server'_weak.
+      apply match_index_all_entries_do_generic_server.
+    - apply match_index_all_entries_state_same_packet_subset.
+    - apply refined_raft_net_invariant_reboot'_weak.
+      apply match_index_all_entries_reboot.
+  Qed.
+
+  Instance miaei : match_index_all_entries_interface.
+  Proof.
+    constructor.
+    apply match_index_all_entries_invariant.
+  Qed.
+End MatchIndexAllEntries.
